\documentclass{article}
\usepackage{amsfonts}
\usepackage{amsmath, fullpage}

\begin{document}

\newcommand{\bC}{\mathbf{C}}
\newcommand{\bF}{\mathbf{F}}
\newcommand{\bI}{\mathbf{I}}
\newcommand{\bP}{\mathbf{P}}
\newcommand{\bR}{\mathbf{R}}
\newcommand{\R}{\mathbb{R}}
\newcommand{\bS}{\mathbf{S}}
\newcommand{\bX}{\mathbf{X}}
\newcommand{\bx}{\mathbf{x}}

\newcommand{\bFt}{\mathbf{F}^t}

\title{Codimensional Corotated Energy Note}
\author{Zhan Zhang}
%\date{\vspace{-5ex}}
\maketitle
\thispagestyle{empty}

\section{Energy}
    \begin{equation}
        E(\bx) = \sum_t\Psi(\bFt(\bx))A^t
    \end{equation}
    \begin{equation}
    \begin{aligned}
        \Psi(\bF(\bx)) &= \mu\,\text{tr}\left[(\bF-\bR(\bF))^T(\bF-\bR(\bF))\right]+\frac{\lambda}{2}(\sqrt{\text{det}(\bF^T\bF)}-1)^2\\
        &=\mu\,\text{tr}\left[\bF^T\bF-2\bS+\bI\right]+\frac{\lambda}{2}(\sqrt{\text{det}(\bF^T\bF)}-1)^2\\
    \end{aligned}
    \end{equation} 
    where, $\bF = \bR(\bF)\,\bS(\bF)$ is the polar deconposition, $\bR^T\bR = \bI\in\R^{2\times2}$. And $\bFt,\bF,\bR\in\R^{3\times2}$, $\bS\in\R^{2\times2}$. 

\section{First-Piola-Kirchhoff Stress}
    \begin{equation}
    \begin{aligned}
        \bP(\bF) &= \frac{\partial\Psi}{\partial\bF}(\bF)\\
        &= \mu\,\frac{\partial}{\partial F_{\alpha\beta}}\left[F_{\gamma\delta}F_{\gamma\delta}-2\text{tr}(\bS)\right]+\lambda(\sqrt{\text{det}(\bF^T\bF)}-1)\frac{\partial \text{det}(\bF^T\bF) /\partial \bF}{2\sqrt{\text{det}(\bF^T\bF)}}\\
        &= 2\mu\bF - 2\mu\,\frac{\partial \, \text{tr}(\bS)}{\partial \bF}+\lambda(J-1)\frac{\partial J}{\partial \bF}\\
        &= 2\mu(\bF-\bR)+\lambda(J-1)J\bF(\bF^T\bF)^{-T}
    \end{aligned}
    \end{equation}

    \subsection{$\frac{\partial \, \text{tr}(\bS)}{\partial \bF}$}
    \begin{equation}
    \begin{aligned}
        \delta\text{tr}(\bS) &= \text{tr}(\delta \bS)\\
        &= \text{tr}(\delta\bR^T\bF) + \text{tr}(\bR^T\delta\bF)\\
        &= \text{tr}(\delta\bR^T\bR\cdot\bS)  + \text{tr}(\bR^T\delta\bF)\\
        &= R_{\alpha\beta}\delta F_{\alpha\beta}
    \end{aligned}
    \end{equation}
    Thus,
    \begin{equation}
        \frac{\partial \, \text{tr}(\bS)}{\partial \bF} = \bR
    \end{equation}

    \subsection{$\frac{\partial J}{\partial \bF}$}
    \begin{equation}
    \begin{aligned}
        \frac{\partial J}{\partial \bF} &= \frac{1}{2J}\frac{\partial J^2}{\partial \bF^T\bF}:\frac{\partial \bF^T\bF}{\partial \bF}\\
        &= \frac{1}{2J}J^2(\bF^T\bF)^{-1}_{\delta\gamma}:\frac{\partial (\bF^T\bF)_{\gamma\delta}}{\partial \bF_{\alpha\beta}} \\
        &= \frac{J}{2}(\bF^T\bF)^{-1}_{\beta\gamma}\cdot2\bF_{\alpha\gamma}\\
        &= J\bF(\bF^T\bF)^{-T}\\ 
    \end{aligned}
    \end{equation}

\section{Energy Denisity Hessian}
    \begin{equation}
    \begin{aligned}
        \bC_{\alpha\gamma\beta\epsilon} &= \frac{\partial^2 \Psi}{\partial \bF_{\alpha\gamma}\partial \bF_{\beta\epsilon}}(\bF) = \frac{\partial \bP_{\alpha\gamma}}{\partial\bF_{\beta\epsilon}}(\bF)\\
        &= 2\mu(\delta_{\alpha\beta}\delta_{\gamma\epsilon}-\frac{\partial \bR_{\alpha\gamma}}{\partial \bF_{\beta\epsilon}})+\lambda\frac{\partial J}{\partial \bF_{\alpha\gamma}}(J\bF(\bF^T\bF)^{-T})_{\beta\epsilon}+\lambda(J-1)\frac{\partial J(\bF(\bF^T\bF)^{-T})_{\alpha\gamma}}{\partial \bF_{\beta\epsilon}}\\
        &= 2\mu(\bI-\frac{\partial \bR_{\alpha\gamma}}{\partial \bF_{\beta\epsilon}})+\lambda(J\bF(\bF^T\bF)^{-T})\otimes (J\bF(\bF^T\bF)^{-T})+\lambda(J-1)\frac{\partial J(\bF(\bF^T\bF)^{-T})_{\alpha\gamma}}{\partial \bF_{\beta\epsilon}}
    \end{aligned}
    \end{equation}
\end{document}
